lookupQuotientContribution mid => low

src/specs/LookupQuotientContribution.ec
@@ -1,3 +1,6 @@
+require import AllCore.
+require import Int.
+require import IntDiv.
 require        Constants.
 require import Modexp.
 require import PurePrimops.
@@ -8,7 +11,7 @@ require import YulPrimops.
 
 module LookupQuotientContribution = {
   proc low(): uint256 = {
-    var ret, betaLookup, gammaLookup, betaPlusOne, betaGamma, _8, _10, _12, lastOmega, _18, zMinusLastOmega, _21, _23, intermediateValue, lnMinusOneAtZ, betaGammaPowered, alphaPower8, _27, subtrahend;
+    var ret, betaLookup, gammaLookup, betaPlusOne, betaGamma, _8, _10, _12, lastOmega, _18, zMinusLastOmega, _21, _23, intermediateValue, lnMinusOneAtZ, betaGammaPowered, alphaPower8, _27, subtrahend : uint256;
     betaLookup <@ Primops.mload(STATE_BETA_LOOKUP_SLOT);
     gammaLookup <@ Primops.mload(STATE_GAMMA_LOOKUP_SLOT);
     betaPlusOne <- (PurePrimops.addmod betaLookup W256.one R_MOD);
@@ -39,6 +42,35 @@ module LookupQuotientContribution = {
     ret <- (PurePrimops.addmod ret (R_MOD - subtrahend) R_MOD);
     return ret;
   }
+
+  proc mid (
+      stateBetaLookupSlot
+      stateGammaLookupSlot
+      statePowerOfAlpha6Slot
+      statePowerOfAlpha7Slot
+      statePowerOfAlpha8Slot
+      proofLookupSPolyOpeningAtZOmegaSlot
+      proofLookupGrandProductOpeningAtZOmegaSlot
+      stateZSlot
+      stateL0AtZSlot
+      stateLnMinusOneAtZSlot
+      : int) = {
+    var betaPlusOne, betaGamma, lastOmega, zMinusLastOmega, betaGammaPowered: int;
+    var f, a6c, a6c', a7c, a8c: int;
+
+    betaPlusOne <- (stateBetaLookupSlot + 1) %% Constants.R;
+    betaGamma <- (stateGammaLookupSlot * betaPlusOne) %% Constants.R;
+    f <- (proofLookupSPolyOpeningAtZOmegaSlot * stateBetaLookupSlot + betaGamma) %% Constants.R;
+    a6c' <- (statePowerOfAlpha6Slot * f * proofLookupGrandProductOpeningAtZOmegaSlot) %% Constants.R;
+    lastOmega <@ Modexp.mid(Constants.OMEGA, (Constants.DOMAIN_SIZE - 1));
+    zMinusLastOmega <- (stateZSlot - lastOmega) %% Constants.R;
+    a6c <- (a6c' * zMinusLastOmega) %% Constants.R; 
+    a7c <- (statePowerOfAlpha7Slot * stateL0AtZSlot) %% Constants.R;
+    betaGammaPowered <@ Modexp.mid(betaGamma, Constants.DOMAIN_SIZE - 1);
+    a8c <- (statePowerOfAlpha8Slot * stateLnMinusOneAtZSlot * betaGammaPowered) %% Constants.R;
+
+    return ((a6c - a7c - a8c) %% Constants.R, betaPlusOne, betaGamma, zMinusLastOmega);
+  }
 }.
 
 lemma lookupQuotientContribution_extracted_equiv_low:
@@ -59,8 +91,665 @@ lemma lookupQuotientContribution_extracted_equiv_low:
       seq 5 2: (#pre /\ usr_zMinusLastOmega{1} = zMinusLastOmega{2}). inline*. wp. skip. rewrite /Constants.R. by progress.
       seq 10 5: (#pre /\ usr_intermediateValue{1} = intermediateValue{2}). inline*. wp. skip. rewrite /Constants.R. by progress.
       seq 5 2: (#pre /\ usr_lnMinusOneAtZ{1} = lnMinusOneAtZ{2}). inline*. wp. skip. rewrite /Constants.R. by progress.
-      seq 2 1: (#pre /\ usr_betaGammaPowered{1} = betaGammaPowered{2}). wp. call modexp_extracted_equiv_low. skip. progress. rewrite /Constants.DOMAIN_SIZE. by progress.
+      seq 2 1: (#pre /\ usr_betaGammaPowered{1} = betaGammaPowered{2}). wp. call modexp_extracted_equiv_low. skip. by progress. 
       seq 3 1: (#pre /\ usr_alphaPower8{1} = alphaPower8{2}). inline*. wp. skip. by progress.
       seq 2 2: (#pre /\ usr_subtrahend{1} = subtrahend{2}). wp. skip. rewrite /Constants.R. by progress.
       wp. skip. rewrite /Constants.R. by progress.
     qed.
+
+section.
+import MemoryMap PurePrimops.
+declare op m : mem.
+
+op lookupQuotientContribution_memory_footprint 
+  (lastOmega
+   betaPlusOne
+   betaGamma
+   zMinusLastOmega v : int)
+  =
+  let m1 = store m STATE_BETA_PLUS_ONE_SLOT (W256.of_int betaPlusOne) in
+  let m2 = store m1 STATE_BETA_GAMMA_PLUS_GAMMA_SLOT (W256.of_int betaGamma) in
+  let m3 = modexp_memory_footprint m2 OMEGA (DOMAIN_SIZE - W256.one) (W256.of_int lastOmega) in
+  let m4 = store m3 STATE_Z_MINUS_LAST_OMEGA_SLOT (W256.of_int zMinusLastOmega) in
+  let m5 = modexp_memory_footprint m4 (W256.of_int betaGamma) (DOMAIN_SIZE - W256.one) (W256.of_int v) in
+  m5.
+
+lemma LookupQuotientContribution_low_equiv_mid (
+stateBetaLookupSlotG
+stateGammaLookupSlotG
+statePowerOfAlpha6SlotG
+statePowerOfAlpha7SlotG
+statePowerOfAlpha8SlotG
+proofLookupSPolyOpeningAtZOmegaSlotG
+proofLookupGrandProductOpeningAtZOmegaSlotG
+stateZSlotG
+stateL0AtZSlotG
+stateLnMinusOneAtZSlotG
+zMinusLastOmegaG : int
+) :
+equiv [LookupQuotientContribution.low ~ LookupQuotientContribution.mid :
+arg{2} =
+  (stateBetaLookupSlotG, stateGammaLookupSlotG, statePowerOfAlpha6SlotG,
+   statePowerOfAlpha7SlotG, statePowerOfAlpha8SlotG, proofLookupSPolyOpeningAtZOmegaSlotG,
+   proofLookupGrandProductOpeningAtZOmegaSlotG, stateZSlotG, stateL0AtZSlotG, stateLnMinusOneAtZSlotG) /\
+Primops.memory{1} = m /\
+!Primops.reverted{1} /\
+W256.to_uint (mload m STATE_BETA_LOOKUP_SLOT) = stateBetaLookupSlotG /\
+W256.to_uint (mload m STATE_GAMMA_LOOKUP_SLOT) = stateGammaLookupSlotG /\
+W256.to_uint (mload m STATE_POWER_OF_ALPHA_6_SLOT) = statePowerOfAlpha6SlotG /\
+W256.to_uint (mload m STATE_POWER_OF_ALPHA_7_SLOT) = statePowerOfAlpha7SlotG /\
+W256.to_uint (mload m STATE_POWER_OF_ALPHA_8_SLOT) = statePowerOfAlpha8SlotG /\
+W256.to_uint (mload m PROOF_LOOKUP_S_POLY_OPENING_AT_Z_OMEGA_SLOT) = proofLookupSPolyOpeningAtZOmegaSlotG /\
+W256.to_uint (mload m PROOF_LOOKUP_GRAND_PRODUCT_OPENING_AT_Z_OMEGA_SLOT) = proofLookupGrandProductOpeningAtZOmegaSlotG /\
+W256.to_uint (mload m STATE_Z_SLOT) = stateZSlotG /\
+W256.to_uint (mload m STATE_L_0_AT_Z_SLOT) = stateL0AtZSlotG /\
+W256.to_uint (mload m STATE_L_N_MINUS_ONE_AT_Z_SLOT) = stateLnMinusOneAtZSlotG /\
+W256.to_uint (mload m STATE_Z_MINUS_LAST_OMEGA_SLOT) = zMinusLastOmegaG
+==>
+!Primops.reverted{1} /\
+exists lastOmega s, 
+Primops.memory{1} = lookupQuotientContribution_memory_footprint lastOmega res{2}.`2 res{2}.`3 res{2}.`4 s /\
+res{2}.`1 = W256.to_uint res{1} /\
+0 <= res{2}.`1 < Constants.R /\
+0 <= res{2}.`2 < Constants.R /\
+0 <= res{2}.`3 < Constants.R /\
+0 <= res{2}.`4 < Constants.R
+].
+proof. proc. simplify.
+seq 2 0: (#pre /\
+  W256.to_uint betaLookup{1} = stateBetaLookupSlotG /\
+  W256.to_uint gammaLookup{1} = stateGammaLookupSlotG).
+call{1} (ConcretePrimops.mload_pspec m STATE_GAMMA_LOOKUP_SLOT).
+call{1} (ConcretePrimops.mload_pspec m STATE_BETA_LOOKUP_SLOT).
+skip. by progress.
+
+seq 2 2 : (#pre /\
+  W256.to_uint betaPlusOne{1} = betaPlusOne{2} /\ betaPlusOne{2} = (stateBetaLookupSlot{2} + 1) %% Constants.R /\
+  W256.to_uint betaGamma{1} = betaGamma{2} /\ betaGamma{2} = (stateGammaLookupSlot{2} * betaPlusOne{2}) %% Constants.R).
+wp. skip. rewrite /addmod /mulmod. progress.
+rewrite H0. by smt. 
+rewrite H0 H1. by smt.
+
+exists* betaPlusOne{1}. elim*=> bpo. exists* betaGamma{1}. elim*=> bg.
+pose m1 := store m STATE_BETA_PLUS_ONE_SLOT bpo.
+pose m2 := store m1 STATE_BETA_GAMMA_PLUS_GAMMA_SLOT bg.
+seq 2 0: (
+!Primops.reverted{1} /\
+bg = betaGamma{1} /\
+bpo = betaPlusOne{1} /\
+stateBetaLookupSlot{2} = stateBetaLookupSlotG /\
+stateGammaLookupSlot{2} = stateGammaLookupSlotG /\
+statePowerOfAlpha6Slot{2} = statePowerOfAlpha6SlotG /\
+statePowerOfAlpha7Slot{2} = statePowerOfAlpha7SlotG /\
+statePowerOfAlpha8Slot{2} = statePowerOfAlpha8SlotG /\
+proofLookupSPolyOpeningAtZOmegaSlot{2} =
+proofLookupSPolyOpeningAtZOmegaSlotG /\
+proofLookupGrandProductOpeningAtZOmegaSlot{2} =
+proofLookupGrandProductOpeningAtZOmegaSlotG /\
+stateZSlot{2} = stateZSlotG /\
+stateL0AtZSlot{2} = stateL0AtZSlotG /\
+stateLnMinusOneAtZSlot{2} = stateLnMinusOneAtZSlotG /\
+to_uint (mload m STATE_BETA_LOOKUP_SLOT) = stateBetaLookupSlotG /\
+to_uint (mload m STATE_GAMMA_LOOKUP_SLOT) = stateGammaLookupSlotG /\
+to_uint (mload m STATE_POWER_OF_ALPHA_6_SLOT) = statePowerOfAlpha6SlotG /\
+to_uint (mload m STATE_POWER_OF_ALPHA_7_SLOT) = statePowerOfAlpha7SlotG /\
+to_uint (mload m STATE_POWER_OF_ALPHA_8_SLOT) = statePowerOfAlpha8SlotG /\
+to_uint (mload m PROOF_LOOKUP_S_POLY_OPENING_AT_Z_OMEGA_SLOT) = proofLookupSPolyOpeningAtZOmegaSlotG /\
+to_uint (mload m PROOF_LOOKUP_GRAND_PRODUCT_OPENING_AT_Z_OMEGA_SLOT) = proofLookupGrandProductOpeningAtZOmegaSlotG /\
+to_uint (mload m STATE_Z_SLOT) = stateZSlotG /\
+to_uint (mload m STATE_L_0_AT_Z_SLOT) = stateL0AtZSlotG /\
+to_uint (mload m STATE_L_N_MINUS_ONE_AT_Z_SLOT) = stateLnMinusOneAtZSlotG /\
+to_uint (mload m STATE_Z_MINUS_LAST_OMEGA_SLOT) = zMinusLastOmegaG /\
+to_uint betaLookup{1} = stateBetaLookupSlotG /\
+to_uint gammaLookup{1} = stateGammaLookupSlotG /\
+to_uint betaPlusOne{1} = betaPlusOne{2} /\
+betaPlusOne{2} = (stateBetaLookupSlot{2} + 1) %% Constants.R /\
+to_uint betaGamma{1} = betaGamma{2} /\
+betaGamma{2} = stateGammaLookupSlot{2} * betaPlusOne{2} %% Constants.R /\
+Primops.memory{1} = m2
+).
+call{1} (ConcretePrimops.mstore_pspec m1 STATE_BETA_GAMMA_PLUS_GAMMA_SLOT bg).
+call{1} (ConcretePrimops.mstore_pspec m STATE_BETA_PLUS_ONE_SLOT bpo).
+skip. by progress.
+
+seq 1 0: (#pre /\ to_uint _8{1} = proofLookupSPolyOpeningAtZOmegaSlot{2}).
+call{1} (ConcretePrimops.mload_pspec m2 PROOF_LOOKUP_S_POLY_OPENING_AT_Z_OMEGA_SLOT).
+skip; progress; rewrite /m2 /m1. 
+rewrite load_store_diff;
+rewrite /PROOF_LOOKUP_S_POLY_OPENING_AT_Z_OMEGA_SLOT /STATE_BETA_GAMMA_PLUS_GAMMA_SLOT; try by auto.
+rewrite load_store_diff;
+rewrite /PROOF_LOOKUP_S_POLY_OPENING_AT_Z_OMEGA_SLOT /STATE_BETA_PLUS_ONE_SLOT; try by smt().
+
+seq 1 0: (#pre /\
+  to_uint ret{1} = (proofLookupSPolyOpeningAtZOmegaSlot{2} * stateBetaLookupSlot{2}) %% Constants.R
+).
+wp. skip. progress. rewrite /mulmod H4 H0. progress. smt.
+seq 1 1:(
+  !Primops.reverted{1} /\
+    bg = betaGamma{1} /\
+    bpo = betaPlusOne{1} /\
+    stateBetaLookupSlot{2} = stateBetaLookupSlotG /\
+    stateGammaLookupSlot{2} = stateGammaLookupSlotG /\
+    statePowerOfAlpha6Slot{2} = statePowerOfAlpha6SlotG /\
+    statePowerOfAlpha7Slot{2} = statePowerOfAlpha7SlotG /\
+    statePowerOfAlpha8Slot{2} = statePowerOfAlpha8SlotG /\
+    proofLookupSPolyOpeningAtZOmegaSlot{2} =
+    proofLookupSPolyOpeningAtZOmegaSlotG /\
+    proofLookupGrandProductOpeningAtZOmegaSlot{2} =
+    proofLookupGrandProductOpeningAtZOmegaSlotG /\
+    stateZSlot{2} = stateZSlotG /\
+    stateL0AtZSlot{2} = stateL0AtZSlotG /\
+    stateLnMinusOneAtZSlot{2} = stateLnMinusOneAtZSlotG /\
+    to_uint (mload m STATE_BETA_LOOKUP_SLOT) = stateBetaLookupSlotG /\
+    to_uint (mload m STATE_GAMMA_LOOKUP_SLOT) = stateGammaLookupSlotG /\
+    to_uint (mload m STATE_POWER_OF_ALPHA_6_SLOT) = statePowerOfAlpha6SlotG /\
+    to_uint (mload m STATE_POWER_OF_ALPHA_7_SLOT) = statePowerOfAlpha7SlotG /\
+    to_uint (mload m STATE_POWER_OF_ALPHA_8_SLOT) = statePowerOfAlpha8SlotG /\
+    to_uint (mload m PROOF_LOOKUP_S_POLY_OPENING_AT_Z_OMEGA_SLOT) =
+    proofLookupSPolyOpeningAtZOmegaSlotG /\
+    to_uint (mload m PROOF_LOOKUP_GRAND_PRODUCT_OPENING_AT_Z_OMEGA_SLOT) =
+    proofLookupGrandProductOpeningAtZOmegaSlotG /\
+    to_uint (mload m STATE_Z_SLOT) = stateZSlotG /\
+    to_uint (mload m STATE_L_0_AT_Z_SLOT) = stateL0AtZSlotG /\
+    to_uint (mload m STATE_L_N_MINUS_ONE_AT_Z_SLOT) = stateLnMinusOneAtZSlotG /\
+    to_uint (mload m STATE_Z_MINUS_LAST_OMEGA_SLOT) = zMinusLastOmegaG /\
+    to_uint betaLookup{1} = stateBetaLookupSlotG /\
+    to_uint gammaLookup{1} = stateGammaLookupSlotG /\
+    to_uint betaPlusOne{1} = betaPlusOne{2} /\
+    betaPlusOne{2} = (stateBetaLookupSlot{2} + 1) %% Constants.R /\
+    to_uint betaGamma{1} = betaGamma{2} /\
+    betaGamma{2} = stateGammaLookupSlot{2} * betaPlusOne{2} %% Constants.R /\
+    Primops.memory{1} = m2 /\
+   to_uint _8{1} = proofLookupSPolyOpeningAtZOmegaSlot{2} /\
+  to_uint ret{1} = f{2} /\
+  f{2} = (proofLookupSPolyOpeningAtZOmegaSlot{2} * stateBetaLookupSlot{2} + betaGamma{2}) %% Constants.R
+).
+wp. skip. progress. rewrite /addmod H5 H3 H2. progress. smt.
+
+seq 1 0: (#pre /\ to_uint _10{1} = proofLookupGrandProductOpeningAtZOmegaSlot{2}).
+call{1} (ConcretePrimops.mload_pspec m2 PROOF_LOOKUP_GRAND_PRODUCT_OPENING_AT_Z_OMEGA_SLOT).
+skip. progress. rewrite /m2 /m1. 
+rewrite load_store_diff;
+rewrite /PROOF_LOOKUP_S_POLY_OPENING_AT_Z_OMEGA_SLOT /STATE_BETA_GAMMA_PLUS_GAMMA_SLOT /PROOF_LOOKUP_GRAND_PRODUCT_OPENING_AT_Z_OMEGA_SLOT /STATE_BETA_PLUS_ONE_SLOT; try by auto.
+rewrite load_store_diff;
+rewrite /PROOF_LOOKUP_S_POLY_OPENING_AT_Z_OMEGA_SLOT /STATE_BETA_PLUS_ONE_SLOT; try by smt().
+
+seq 2 0:(
+  !Primops.reverted{1} /\
+   bg = betaGamma{1} /\
+   bpo = betaPlusOne{1} /\
+   stateBetaLookupSlot{2} = stateBetaLookupSlotG /\
+   stateGammaLookupSlot{2} = stateGammaLookupSlotG /\
+   statePowerOfAlpha6Slot{2} = statePowerOfAlpha6SlotG /\
+   statePowerOfAlpha7Slot{2} = statePowerOfAlpha7SlotG /\
+   statePowerOfAlpha8Slot{2} = statePowerOfAlpha8SlotG /\
+   proofLookupSPolyOpeningAtZOmegaSlot{2} =
+   proofLookupSPolyOpeningAtZOmegaSlotG /\
+   proofLookupGrandProductOpeningAtZOmegaSlot{2} =
+   proofLookupGrandProductOpeningAtZOmegaSlotG /\
+   stateZSlot{2} = stateZSlotG /\
+   stateL0AtZSlot{2} = stateL0AtZSlotG /\
+   stateLnMinusOneAtZSlot{2} = stateLnMinusOneAtZSlotG /\
+   to_uint (mload m STATE_BETA_LOOKUP_SLOT) = stateBetaLookupSlotG /\
+   to_uint (mload m STATE_GAMMA_LOOKUP_SLOT) = stateGammaLookupSlotG /\
+   to_uint (mload m STATE_POWER_OF_ALPHA_6_SLOT) = statePowerOfAlpha6SlotG /\
+   to_uint (mload m STATE_POWER_OF_ALPHA_7_SLOT) = statePowerOfAlpha7SlotG /\
+   to_uint (mload m STATE_POWER_OF_ALPHA_8_SLOT) = statePowerOfAlpha8SlotG /\
+   to_uint (mload m PROOF_LOOKUP_S_POLY_OPENING_AT_Z_OMEGA_SLOT) =
+   proofLookupSPolyOpeningAtZOmegaSlotG /\
+   to_uint (mload m PROOF_LOOKUP_GRAND_PRODUCT_OPENING_AT_Z_OMEGA_SLOT) =
+   proofLookupGrandProductOpeningAtZOmegaSlotG /\
+   to_uint (mload m STATE_Z_SLOT) = stateZSlotG /\
+   to_uint (mload m STATE_L_0_AT_Z_SLOT) = stateL0AtZSlotG /\
+   to_uint (mload m STATE_L_N_MINUS_ONE_AT_Z_SLOT) = stateLnMinusOneAtZSlotG /\
+   to_uint (mload m STATE_Z_MINUS_LAST_OMEGA_SLOT) = zMinusLastOmegaG /\
+   to_uint betaLookup{1} = stateBetaLookupSlotG /\
+   to_uint gammaLookup{1} = stateGammaLookupSlotG /\
+   to_uint betaPlusOne{1} = betaPlusOne{2} /\
+   betaPlusOne{2} = (stateBetaLookupSlot{2} + 1) %% Constants.R /\
+   to_uint betaGamma{1} = betaGamma{2} /\
+   betaGamma{2} = stateGammaLookupSlot{2} * betaPlusOne{2} %% Constants.R /\
+   Primops.memory{1} = m2 /\
+   to_uint _8{1} = proofLookupSPolyOpeningAtZOmegaSlot{2} /\
+   f{2} = (proofLookupSPolyOpeningAtZOmegaSlot{2} * stateBetaLookupSlot{2} + betaGamma{2}) %% Constants.R /\
+   to_uint _10{1} = proofLookupGrandProductOpeningAtZOmegaSlot{2} /\
+   to_uint ret{1} = (f{2} * proofLookupGrandProductOpeningAtZOmegaSlot{2}) %% Constants.R /\
+   to_uint _12{1} = statePowerOfAlpha6Slot{2}
+).
+sp.
+call{1} (ConcretePrimops.mload_pspec m2 STATE_POWER_OF_ALPHA_6_SLOT).
+skip. progress. rewrite /mulmod. progress. rewrite H5 H6. smt.
+rewrite /m2 /m1. 
+rewrite load_store_diff;
+rewrite /PROOF_LOOKUP_S_POLY_OPENING_AT_Z_OMEGA_SLOT /STATE_BETA_GAMMA_PLUS_GAMMA_SLOT /PROOF_LOOKUP_GRAND_PRODUCT_OPENING_AT_Z_OMEGA_SLOT /STATE_BETA_PLUS_ONE_SLOT /STATE_POWER_OF_ALPHA_6_SLOT; try by auto.
+rewrite load_store_diff;
+rewrite /PROOF_LOOKUP_S_POLY_OPENING_AT_Z_OMEGA_SLOT /STATE_BETA_PLUS_ONE_SLOT; try by smt().
+
+seq 1 1: (
+  !Primops.reverted{1} /\
+  bg = betaGamma{1} /\
+  bpo = betaPlusOne{1} /\
+  stateBetaLookupSlot{2} = stateBetaLookupSlotG /\
+  stateGammaLookupSlot{2} = stateGammaLookupSlotG /\
+  statePowerOfAlpha6Slot{2} = statePowerOfAlpha6SlotG /\
+  statePowerOfAlpha7Slot{2} = statePowerOfAlpha7SlotG /\
+  statePowerOfAlpha8Slot{2} = statePowerOfAlpha8SlotG /\
+  proofLookupSPolyOpeningAtZOmegaSlot{2} =
+  proofLookupSPolyOpeningAtZOmegaSlotG /\
+  proofLookupGrandProductOpeningAtZOmegaSlot{2} =
+  proofLookupGrandProductOpeningAtZOmegaSlotG /\
+  stateZSlot{2} = stateZSlotG /\
+  stateL0AtZSlot{2} = stateL0AtZSlotG /\
+  stateLnMinusOneAtZSlot{2} = stateLnMinusOneAtZSlotG /\
+  to_uint (mload m STATE_BETA_LOOKUP_SLOT) = stateBetaLookupSlotG /\
+  to_uint (mload m STATE_GAMMA_LOOKUP_SLOT) = stateGammaLookupSlotG /\
+  to_uint (mload m STATE_POWER_OF_ALPHA_6_SLOT) = statePowerOfAlpha6SlotG /\
+  to_uint (mload m STATE_POWER_OF_ALPHA_7_SLOT) = statePowerOfAlpha7SlotG /\
+  to_uint (mload m STATE_POWER_OF_ALPHA_8_SLOT) = statePowerOfAlpha8SlotG /\
+  to_uint (mload m PROOF_LOOKUP_S_POLY_OPENING_AT_Z_OMEGA_SLOT) =
+  proofLookupSPolyOpeningAtZOmegaSlotG /\
+  to_uint (mload m PROOF_LOOKUP_GRAND_PRODUCT_OPENING_AT_Z_OMEGA_SLOT) =
+  proofLookupGrandProductOpeningAtZOmegaSlotG /\
+  to_uint (mload m STATE_Z_SLOT) = stateZSlotG /\
+  to_uint (mload m STATE_L_0_AT_Z_SLOT) = stateL0AtZSlotG /\
+  to_uint (mload m STATE_L_N_MINUS_ONE_AT_Z_SLOT) = stateLnMinusOneAtZSlotG /\
+  to_uint (mload m STATE_Z_MINUS_LAST_OMEGA_SLOT) = zMinusLastOmegaG /\
+  to_uint betaLookup{1} = stateBetaLookupSlotG /\
+  to_uint gammaLookup{1} = stateGammaLookupSlotG /\
+  to_uint betaPlusOne{1} = betaPlusOne{2} /\
+  betaPlusOne{2} = (stateBetaLookupSlot{2} + 1) %% Constants.R /\
+  to_uint betaGamma{1} = betaGamma{2} /\
+  betaGamma{2} = stateGammaLookupSlot{2} * betaPlusOne{2} %% Constants.R /\
+  Primops.memory{1} = m2 /\
+  to_uint _8{1} = proofLookupSPolyOpeningAtZOmegaSlot{2} /\
+  f{2} = (proofLookupSPolyOpeningAtZOmegaSlot{2} * stateBetaLookupSlot{2} + betaGamma{2}) %% Constants.R /\
+  to_uint _10{1} = proofLookupGrandProductOpeningAtZOmegaSlot{2} /\
+  to_uint _12{1} = statePowerOfAlpha6Slot{2} /\
+  to_uint ret{1} = a6c'{2} /\
+  a6c'{2} = (statePowerOfAlpha6Slot{2} * f{2} * proofLookupGrandProductOpeningAtZOmegaSlot{2}) %% Constants.R
+).
+wp. skip. progress. rewrite /mulmod. progress.
+rewrite W256.to_uint_small. progress. by smt. by smt.
+rewrite H6 H7. rewrite W256.to_uint_small. progress. by smt.
+
+seq 1 1:(
+  !Primops.reverted{1} /\
+  bg = betaGamma{1} /\
+  bpo = betaPlusOne{1} /\
+  stateBetaLookupSlot{2} = stateBetaLookupSlotG /\
+  stateGammaLookupSlot{2} = stateGammaLookupSlotG /\
+  statePowerOfAlpha6Slot{2} = statePowerOfAlpha6SlotG /\
+  statePowerOfAlpha7Slot{2} = statePowerOfAlpha7SlotG /\
+  statePowerOfAlpha8Slot{2} = statePowerOfAlpha8SlotG /\
+  proofLookupSPolyOpeningAtZOmegaSlot{2} =
+  proofLookupSPolyOpeningAtZOmegaSlotG /\
+  proofLookupGrandProductOpeningAtZOmegaSlot{2} =
+  proofLookupGrandProductOpeningAtZOmegaSlotG /\
+  stateZSlot{2} = stateZSlotG /\
+  stateL0AtZSlot{2} = stateL0AtZSlotG /\
+  stateLnMinusOneAtZSlot{2} = stateLnMinusOneAtZSlotG /\
+  to_uint (mload m STATE_BETA_LOOKUP_SLOT) = stateBetaLookupSlotG /\
+  to_uint (mload m STATE_GAMMA_LOOKUP_SLOT) = stateGammaLookupSlotG /\
+  to_uint (mload m STATE_POWER_OF_ALPHA_6_SLOT) = statePowerOfAlpha6SlotG /\
+  to_uint (mload m STATE_POWER_OF_ALPHA_7_SLOT) = statePowerOfAlpha7SlotG /\
+  to_uint (mload m STATE_POWER_OF_ALPHA_8_SLOT) = statePowerOfAlpha8SlotG /\
+  to_uint (mload m PROOF_LOOKUP_S_POLY_OPENING_AT_Z_OMEGA_SLOT) =
+  proofLookupSPolyOpeningAtZOmegaSlotG /\
+  to_uint (mload m PROOF_LOOKUP_GRAND_PRODUCT_OPENING_AT_Z_OMEGA_SLOT) =
+  proofLookupGrandProductOpeningAtZOmegaSlotG /\
+  to_uint (mload m STATE_Z_SLOT) = stateZSlotG /\
+  to_uint (mload m STATE_L_0_AT_Z_SLOT) = stateL0AtZSlotG /\
+  to_uint (mload m STATE_L_N_MINUS_ONE_AT_Z_SLOT) = stateLnMinusOneAtZSlotG /\
+  to_uint (mload m STATE_Z_MINUS_LAST_OMEGA_SLOT) = zMinusLastOmegaG /\
+  to_uint betaLookup{1} = stateBetaLookupSlotG /\
+  to_uint gammaLookup{1} = stateGammaLookupSlotG /\
+  to_uint betaPlusOne{1} = betaPlusOne{2} /\
+  betaPlusOne{2} = (stateBetaLookupSlot{2} + 1) %% Constants.R /\
+  to_uint betaGamma{1} = betaGamma{2} /\
+  betaGamma{2} = stateGammaLookupSlot{2} * betaPlusOne{2} %% Constants.R /\
+  to_uint _8{1} = proofLookupSPolyOpeningAtZOmegaSlot{2} /\
+  f{2} =
+  (proofLookupSPolyOpeningAtZOmegaSlot{2} * stateBetaLookupSlot{2} +
+   betaGamma{2}) %%
+  Constants.R /\
+  to_uint _10{1} = proofLookupGrandProductOpeningAtZOmegaSlot{2} /\
+  to_uint _12{1} = statePowerOfAlpha6Slot{2} /\
+  to_uint ret{1} = a6c'{2} /\
+  a6c'{2} =
+  statePowerOfAlpha6Slot{2} * f{2} *
+  proofLookupGrandProductOpeningAtZOmegaSlot{2} %% Constants.R /\
+  Primops.memory{1} = modexp_memory_footprint m2 OMEGA (DOMAIN_SIZE - W256.one) lastOmega{1} /\
+  to_uint lastOmega{1} = lastOmega{2} /\
+  0 <= lastOmega{2} < Constants.R
+).
+call (modexp_low_equiv_mid m2 OMEGA (DOMAIN_SIZE - W256.one)).
+skip. progress. rewrite /OMEGA. by smt(). rewrite /DOMAIN_SIZE. by progress.
+exists* lastOmega{1}. elim* => ol.
+pose m3 := modexp_memory_footprint m2 OMEGA (DOMAIN_SIZE - W256.one) ol.
+
+seq 1 0 : (#pre /\ to_uint _18{1} = stateZSlot{2}).
+call{1} (ConcretePrimops.mload_pspec m3 STATE_Z_SLOT).
+skip. progress. rewrite /m3 /m2 /m1 /modexp_memory_footprint. progress.  
+rewrite load_store_diff /STATE_Z_SLOT. by progress. by progress.
+do 6! (rewrite load_store_diff; try by progress). 
+rewrite /STATE_BETA_GAMMA_PLUS_GAMMA_SLOT. by progress.
+rewrite load_store_diff /STATE_BETA_PLUS_ONE_SLOT. by progress. by progress. by smt().
+
+seq 1 1: (#pre /\
+  to_uint zMinusLastOmega{1} = zMinusLastOmega{2} /\
+  zMinusLastOmega{2} = (stateZSlot{2} - lastOmega{2}) %% Constants.R).
+wp. skip. progress. rewrite /addmod H10. progress.
+rewrite W256.to_uint_small. progress. smt. smt. 
+have ->: (to_uint (mload m STATE_Z_SLOT) - to_uint lastOmega{1}) %% Constants.R = (to_uint (mload m STATE_Z_SLOT) + (Constants.R - to_uint lastOmega{1})) %% Constants.R. by smt().
+rewrite to_uintB. by smt. by smt.
+
+exists* zMinusLastOmega{1}. elim* => zmlo.
+pose m4 := store m3 STATE_Z_MINUS_LAST_OMEGA_SLOT zmlo.
+seq 1 0:(
+!Primops.reverted{1} /\
+  zmlo = zMinusLastOmega{1} /\
+  ol = lastOmega{1} /\
+    bg = betaGamma{1} /\
+    bpo = betaPlusOne{1} /\
+    stateBetaLookupSlot{2} = stateBetaLookupSlotG /\
+    stateGammaLookupSlot{2} = stateGammaLookupSlotG /\
+    statePowerOfAlpha6Slot{2} = statePowerOfAlpha6SlotG /\
+    statePowerOfAlpha7Slot{2} = statePowerOfAlpha7SlotG /\
+    statePowerOfAlpha8Slot{2} = statePowerOfAlpha8SlotG /\
+    proofLookupSPolyOpeningAtZOmegaSlot{2} =
+    proofLookupSPolyOpeningAtZOmegaSlotG /\
+    proofLookupGrandProductOpeningAtZOmegaSlot{2} =
+    proofLookupGrandProductOpeningAtZOmegaSlotG /\
+    stateZSlot{2} = stateZSlotG /\
+    stateL0AtZSlot{2} = stateL0AtZSlotG /\
+    stateLnMinusOneAtZSlot{2} = stateLnMinusOneAtZSlotG /\
+    to_uint (mload m STATE_BETA_LOOKUP_SLOT) = stateBetaLookupSlotG /\
+    to_uint (mload m STATE_GAMMA_LOOKUP_SLOT) = stateGammaLookupSlotG /\
+    to_uint (mload m STATE_POWER_OF_ALPHA_6_SLOT) = statePowerOfAlpha6SlotG /\
+    to_uint (mload m STATE_POWER_OF_ALPHA_7_SLOT) = statePowerOfAlpha7SlotG /\
+    to_uint (mload m STATE_POWER_OF_ALPHA_8_SLOT) = statePowerOfAlpha8SlotG /\
+    to_uint (mload m PROOF_LOOKUP_S_POLY_OPENING_AT_Z_OMEGA_SLOT) =
+    proofLookupSPolyOpeningAtZOmegaSlotG /\
+    to_uint (mload m PROOF_LOOKUP_GRAND_PRODUCT_OPENING_AT_Z_OMEGA_SLOT) =
+    proofLookupGrandProductOpeningAtZOmegaSlotG /\
+    to_uint (mload m STATE_Z_SLOT) = stateZSlotG /\
+    to_uint (mload m STATE_L_0_AT_Z_SLOT) = stateL0AtZSlotG /\
+    to_uint (mload m STATE_L_N_MINUS_ONE_AT_Z_SLOT) = stateLnMinusOneAtZSlotG /\
+    to_uint (mload m STATE_Z_MINUS_LAST_OMEGA_SLOT) = zMinusLastOmegaG /\
+    to_uint betaLookup{1} = stateBetaLookupSlotG /\
+    to_uint gammaLookup{1} = stateGammaLookupSlotG /\
+    to_uint betaPlusOne{1} = betaPlusOne{2} /\
+    betaPlusOne{2} = (stateBetaLookupSlot{2} + 1) %% Constants.R /\
+    to_uint betaGamma{1} = betaGamma{2} /\
+    betaGamma{2} = stateGammaLookupSlot{2} * betaPlusOne{2} %% Constants.R /\
+    to_uint _8{1} = proofLookupSPolyOpeningAtZOmegaSlot{2} /\
+    f{2} =
+    (proofLookupSPolyOpeningAtZOmegaSlot{2} * stateBetaLookupSlot{2} +
+     betaGamma{2}) %%
+    Constants.R /\
+    to_uint _10{1} = proofLookupGrandProductOpeningAtZOmegaSlot{2} /\
+    to_uint _12{1} = statePowerOfAlpha6Slot{2} /\
+    to_uint ret{1} = a6c'{2} /\
+    a6c'{2} =
+    statePowerOfAlpha6Slot{2} * f{2} *
+    proofLookupGrandProductOpeningAtZOmegaSlot{2} %% Constants.R /\
+    to_uint lastOmega{1} = lastOmega{2} /\
+    0 <= lastOmega{2} && lastOmega{2} < Constants.R /\
+   to_uint _18{1} = stateZSlot{2} /\
+  to_uint zMinusLastOmega{1} = zMinusLastOmega{2} /\
+  zMinusLastOmega{2} = (stateZSlot{2} - lastOmega{2}) %% Constants.R /\
+  Primops.memory{1} = m4
+).
+call{1} (ConcretePrimops.mstore_pspec m3 STATE_Z_MINUS_LAST_OMEGA_SLOT zmlo).
+skip. by progress.
+
+seq 3 1:(
+  !Primops.reverted{1} /\
+  zmlo = zMinusLastOmega{1} /\
+  ol = lastOmega{1} /\
+  bg = betaGamma{1} /\
+  bpo = betaPlusOne{1} /\
+  stateBetaLookupSlot{2} = stateBetaLookupSlotG /\
+  stateGammaLookupSlot{2} = stateGammaLookupSlotG /\
+  statePowerOfAlpha6Slot{2} = statePowerOfAlpha6SlotG /\
+  statePowerOfAlpha7Slot{2} = statePowerOfAlpha7SlotG /\
+  statePowerOfAlpha8Slot{2} = statePowerOfAlpha8SlotG /\
+  proofLookupSPolyOpeningAtZOmegaSlot{2} =
+  proofLookupSPolyOpeningAtZOmegaSlotG /\
+  proofLookupGrandProductOpeningAtZOmegaSlot{2} =
+  proofLookupGrandProductOpeningAtZOmegaSlotG /\
+  stateZSlot{2} = stateZSlotG /\
+  stateL0AtZSlot{2} = stateL0AtZSlotG /\
+  stateLnMinusOneAtZSlot{2} = stateLnMinusOneAtZSlotG /\
+  to_uint (mload m STATE_BETA_LOOKUP_SLOT) = stateBetaLookupSlotG /\
+  to_uint (mload m STATE_GAMMA_LOOKUP_SLOT) = stateGammaLookupSlotG /\
+  to_uint (mload m STATE_POWER_OF_ALPHA_6_SLOT) = statePowerOfAlpha6SlotG /\
+  to_uint (mload m STATE_POWER_OF_ALPHA_7_SLOT) = statePowerOfAlpha7SlotG /\
+  to_uint (mload m STATE_POWER_OF_ALPHA_8_SLOT) = statePowerOfAlpha8SlotG /\
+  to_uint (mload m PROOF_LOOKUP_S_POLY_OPENING_AT_Z_OMEGA_SLOT) =
+  proofLookupSPolyOpeningAtZOmegaSlotG /\
+  to_uint (mload m PROOF_LOOKUP_GRAND_PRODUCT_OPENING_AT_Z_OMEGA_SLOT) =
+  proofLookupGrandProductOpeningAtZOmegaSlotG /\
+  to_uint (mload m STATE_Z_SLOT) = stateZSlotG /\
+  to_uint (mload m STATE_L_0_AT_Z_SLOT) = stateL0AtZSlotG /\
+  to_uint (mload m STATE_L_N_MINUS_ONE_AT_Z_SLOT) = stateLnMinusOneAtZSlotG /\
+  to_uint (mload m STATE_Z_MINUS_LAST_OMEGA_SLOT) = zMinusLastOmegaG /\
+  to_uint betaLookup{1} = stateBetaLookupSlotG /\
+  to_uint gammaLookup{1} = stateGammaLookupSlotG /\
+  to_uint betaPlusOne{1} = betaPlusOne{2} /\
+  betaPlusOne{2} = (stateBetaLookupSlot{2} + 1) %% Constants.R /\
+  to_uint betaGamma{1} = betaGamma{2} /\
+  betaGamma{2} = stateGammaLookupSlot{2} * betaPlusOne{2} %% Constants.R /\
+  to_uint _8{1} = proofLookupSPolyOpeningAtZOmegaSlot{2} /\
+  f{2} =
+  (proofLookupSPolyOpeningAtZOmegaSlot{2} * stateBetaLookupSlot{2} +
+   betaGamma{2}) %%
+  Constants.R /\
+  to_uint _10{1} = proofLookupGrandProductOpeningAtZOmegaSlot{2} /\
+  to_uint _12{1} = statePowerOfAlpha6Slot{2} /\
+  a6c'{2} =
+  statePowerOfAlpha6Slot{2} * f{2} *
+  proofLookupGrandProductOpeningAtZOmegaSlot{2} %% Constants.R /\
+  to_uint lastOmega{1} = lastOmega{2} /\
+  0 <= lastOmega{2} &&
+  lastOmega{2} < Constants.R /\
+  to_uint _18{1} = stateZSlot{2} /\
+  to_uint zMinusLastOmega{1} = zMinusLastOmega{2} /\
+  zMinusLastOmega{2} = (stateZSlot{2} - lastOmega{2}) %% Constants.R /\
+  Primops.memory{1} = m4 /\
+  to_uint ret{1} = a6c{2} /\ a6c{2} = (a6c'{2} * zMinusLastOmega{2}) %% Constants.R /\
+  to_uint _21{1} = statePowerOfAlpha7Slot{2} /\
+  to_uint _23{1} = stateL0AtZSlot{2}
+).
+sp.
+call{1} (ConcretePrimops.mload_pspec m4 STATE_L_0_AT_Z_SLOT).
+call{1} (ConcretePrimops.mload_pspec m4 STATE_POWER_OF_ALPHA_7_SLOT).
+skip. progress. rewrite /mulmod. progress. rewrite W256.to_uint_small. progress. smt. smt. smt.
+rewrite /m4 /m3 /m2 /m1 /modexp_memory_footprint. progress.  
+rewrite load_store_diff /STATE_POWER_OF_ALPHA_7_SLOT /STATE_Z_MINUS_LAST_OMEGA_SLOT. by progress. by progress.
+do 7! (rewrite load_store_diff; try by progress). 
+rewrite /STATE_BETA_GAMMA_PLUS_GAMMA_SLOT. by progress.
+rewrite load_store_diff /STATE_BETA_PLUS_ONE_SLOT. by smt(). by smt(). by smt().
+rewrite /m4 /m3 /m2 /m1 /modexp_memory_footprint. progress.  
+rewrite load_store_diff /STATE_POWER_OF_ALPHA_7_SLOT /STATE_Z_MINUS_LAST_OMEGA_SLOT /STATE_L_0_AT_Z_SLOT. by progress. by progress.
+do 7! (rewrite load_store_diff; try by progress). 
+rewrite /STATE_BETA_GAMMA_PLUS_GAMMA_SLOT. by progress.
+rewrite load_store_diff /STATE_BETA_PLUS_ONE_SLOT. by smt(). by smt(). by smt().
+
+seq 1 1: (#pre /\
+  to_uint intermediateValue{1} = a7c{2} /\
+  a7c{2} = (statePowerOfAlpha7Slot{2} * stateL0AtZSlot{2}) %% Constants.R).
+wp. skip. rewrite /mulmod. progress. rewrite W256.to_uint_small. progress. smt. smt. rewrite H12 H13. smt. 
+
+seq 1 0:(
+  !Primops.reverted{1} /\
+   zmlo = zMinusLastOmega{1} /\
+   ol = lastOmega{1} /\
+   bg = betaGamma{1} /\
+   bpo = betaPlusOne{1} /\
+   stateBetaLookupSlot{2} = stateBetaLookupSlotG /\
+   stateGammaLookupSlot{2} = stateGammaLookupSlotG /\
+   statePowerOfAlpha6Slot{2} = statePowerOfAlpha6SlotG /\
+   statePowerOfAlpha7Slot{2} = statePowerOfAlpha7SlotG /\
+   statePowerOfAlpha8Slot{2} = statePowerOfAlpha8SlotG /\
+   proofLookupSPolyOpeningAtZOmegaSlot{2} =
+   proofLookupSPolyOpeningAtZOmegaSlotG /\
+   proofLookupGrandProductOpeningAtZOmegaSlot{2} =
+   proofLookupGrandProductOpeningAtZOmegaSlotG /\
+   stateZSlot{2} = stateZSlotG /\
+   stateL0AtZSlot{2} = stateL0AtZSlotG /\
+   stateLnMinusOneAtZSlot{2} = stateLnMinusOneAtZSlotG /\
+   to_uint (mload m STATE_BETA_LOOKUP_SLOT) = stateBetaLookupSlotG /\
+   to_uint (mload m STATE_GAMMA_LOOKUP_SLOT) = stateGammaLookupSlotG /\
+   to_uint (mload m STATE_POWER_OF_ALPHA_6_SLOT) = statePowerOfAlpha6SlotG /\
+   to_uint (mload m STATE_POWER_OF_ALPHA_7_SLOT) = statePowerOfAlpha7SlotG /\
+   to_uint (mload m STATE_POWER_OF_ALPHA_8_SLOT) = statePowerOfAlpha8SlotG /\
+   to_uint (mload m PROOF_LOOKUP_S_POLY_OPENING_AT_Z_OMEGA_SLOT) =
+   proofLookupSPolyOpeningAtZOmegaSlotG /\
+   to_uint (mload m PROOF_LOOKUP_GRAND_PRODUCT_OPENING_AT_Z_OMEGA_SLOT) =
+   proofLookupGrandProductOpeningAtZOmegaSlotG /\
+   to_uint (mload m STATE_Z_SLOT) = stateZSlotG /\
+   to_uint (mload m STATE_L_0_AT_Z_SLOT) = stateL0AtZSlotG /\
+   to_uint (mload m STATE_L_N_MINUS_ONE_AT_Z_SLOT) = stateLnMinusOneAtZSlotG /\
+   to_uint (mload m STATE_Z_MINUS_LAST_OMEGA_SLOT) = zMinusLastOmegaG /\
+   to_uint betaLookup{1} = stateBetaLookupSlotG /\
+   to_uint gammaLookup{1} = stateGammaLookupSlotG /\
+   to_uint betaPlusOne{1} = betaPlusOne{2} /\
+   betaPlusOne{2} = (stateBetaLookupSlot{2} + 1) %% Constants.R /\
+   to_uint betaGamma{1} = betaGamma{2} /\
+   betaGamma{2} = stateGammaLookupSlot{2} * betaPlusOne{2} %% Constants.R /\
+   to_uint _8{1} = proofLookupSPolyOpeningAtZOmegaSlot{2} /\
+   f{2} =
+   (proofLookupSPolyOpeningAtZOmegaSlot{2} * stateBetaLookupSlot{2} +
+    betaGamma{2}) %%
+   Constants.R /\
+   to_uint _10{1} = proofLookupGrandProductOpeningAtZOmegaSlot{2} /\
+   to_uint _12{1} = statePowerOfAlpha6Slot{2} /\
+   a6c'{2} =
+   statePowerOfAlpha6Slot{2} * f{2} *
+   proofLookupGrandProductOpeningAtZOmegaSlot{2} %% Constants.R /\
+   to_uint lastOmega{1} = lastOmega{2} /\
+   0 <= lastOmega{2} &&
+   lastOmega{2} < Constants.R /\
+   to_uint _18{1} = stateZSlot{2} /\
+   to_uint zMinusLastOmega{1} = zMinusLastOmega{2} /\
+   zMinusLastOmega{2} = (stateZSlot{2} - lastOmega{2}) %% Constants.R /\
+   Primops.memory{1} = m4 /\
+   a6c{2} = (a6c'{2} * zMinusLastOmega{2}) %% Constants.R /\
+   to_uint _21{1} = statePowerOfAlpha7Slot{2} /\
+   to_uint _23{1} = stateL0AtZSlot{2} /\
+  to_uint intermediateValue{1} = a7c{2} /\
+  a7c{2} = (statePowerOfAlpha7Slot{2} * stateL0AtZSlot{2}) %% Constants.R /\
+   to_uint ret{1} = (a6c{2} - a7c{2}) %% Constants.R
+).
+wp. skip. rewrite /addmod. progress.
+rewrite W256.to_uint_small. progress. by smt. by smt.
+have ->: (to_uint ret{1} - to_uint intermediateValue{1}) %% Constants.R = (to_uint ret{1} + (Constants.R - to_uint intermediateValue{1})) %% Constants.R. smt().
+rewrite to_uintB. smt timeout=10. smt.
+
+seq 1 0: (#pre /\ to_uint lnMinusOneAtZ{1} = stateLnMinusOneAtZSlot{2}).
+call{1} (ConcretePrimops.mload_pspec m4 STATE_L_N_MINUS_ONE_AT_Z_SLOT).
+skip. progress. rewrite /m4 /m3 /m2 /m1 /modexp_memory_footprint. progress.  
+rewrite load_store_diff /STATE_POWER_OF_ALPHA_7_SLOT /STATE_Z_MINUS_LAST_OMEGA_SLOT /STATE_L_N_MINUS_ONE_AT_Z_SLOT. by progress. by progress.
+do 7! (rewrite load_store_diff; try by progress). 
+rewrite /STATE_BETA_GAMMA_PLUS_GAMMA_SLOT. by progress.
+rewrite load_store_diff /STATE_BETA_PLUS_ONE_SLOT. by smt(). by smt(). by smt().
+
+seq 1 1: (
+   !Primops.reverted{1} /\
+   zmlo = zMinusLastOmega{1} /\
+   ol = lastOmega{1} /\
+   bg = betaGamma{1} /\
+   bpo = betaPlusOne{1} /\
+   stateBetaLookupSlot{2} = stateBetaLookupSlotG /\
+   stateGammaLookupSlot{2} = stateGammaLookupSlotG /\
+   statePowerOfAlpha6Slot{2} = statePowerOfAlpha6SlotG /\
+   statePowerOfAlpha7Slot{2} = statePowerOfAlpha7SlotG /\
+   statePowerOfAlpha8Slot{2} = statePowerOfAlpha8SlotG /\
+   proofLookupSPolyOpeningAtZOmegaSlot{2} =
+   proofLookupSPolyOpeningAtZOmegaSlotG /\
+   proofLookupGrandProductOpeningAtZOmegaSlot{2} =
+   proofLookupGrandProductOpeningAtZOmegaSlotG /\
+   stateZSlot{2} = stateZSlotG /\
+   stateL0AtZSlot{2} = stateL0AtZSlotG /\
+   stateLnMinusOneAtZSlot{2} = stateLnMinusOneAtZSlotG /\
+   to_uint (mload m STATE_BETA_LOOKUP_SLOT) = stateBetaLookupSlotG /\
+   to_uint (mload m STATE_GAMMA_LOOKUP_SLOT) = stateGammaLookupSlotG /\
+   to_uint (mload m STATE_POWER_OF_ALPHA_6_SLOT) = statePowerOfAlpha6SlotG /\
+   to_uint (mload m STATE_POWER_OF_ALPHA_7_SLOT) = statePowerOfAlpha7SlotG /\
+   to_uint (mload m STATE_POWER_OF_ALPHA_8_SLOT) = statePowerOfAlpha8SlotG /\
+   to_uint (mload m PROOF_LOOKUP_S_POLY_OPENING_AT_Z_OMEGA_SLOT) =
+   proofLookupSPolyOpeningAtZOmegaSlotG /\
+   to_uint (mload m PROOF_LOOKUP_GRAND_PRODUCT_OPENING_AT_Z_OMEGA_SLOT) =
+   proofLookupGrandProductOpeningAtZOmegaSlotG /\
+   to_uint (mload m STATE_Z_SLOT) = stateZSlotG /\
+   to_uint (mload m STATE_L_0_AT_Z_SLOT) = stateL0AtZSlotG /\
+   to_uint (mload m STATE_L_N_MINUS_ONE_AT_Z_SLOT) = stateLnMinusOneAtZSlotG /\
+   to_uint (mload m STATE_Z_MINUS_LAST_OMEGA_SLOT) = zMinusLastOmegaG /\
+   to_uint betaLookup{1} = stateBetaLookupSlotG /\
+   to_uint gammaLookup{1} = stateGammaLookupSlotG /\
+   to_uint betaPlusOne{1} = betaPlusOne{2} /\
+   betaPlusOne{2} = (stateBetaLookupSlot{2} + 1) %% Constants.R /\
+   to_uint betaGamma{1} = betaGamma{2} /\
+   betaGamma{2} = stateGammaLookupSlot{2} * betaPlusOne{2} %% Constants.R /\
+   to_uint _8{1} = proofLookupSPolyOpeningAtZOmegaSlot{2} /\
+   f{2} =
+   (proofLookupSPolyOpeningAtZOmegaSlot{2} * stateBetaLookupSlot{2} +
+    betaGamma{2}) %%
+   Constants.R /\
+   to_uint _10{1} = proofLookupGrandProductOpeningAtZOmegaSlot{2} /\
+   to_uint _12{1} = statePowerOfAlpha6Slot{2} /\
+   a6c'{2} =
+   statePowerOfAlpha6Slot{2} * f{2} *
+   proofLookupGrandProductOpeningAtZOmegaSlot{2} %% Constants.R /\
+   to_uint lastOmega{1} = lastOmega{2} /\
+   0 <= lastOmega{2} &&
+   lastOmega{2} < Constants.R /\
+   to_uint _18{1} = stateZSlot{2} /\
+   to_uint zMinusLastOmega{1} = zMinusLastOmega{2} /\
+   zMinusLastOmega{2} = (stateZSlot{2} - lastOmega{2}) %% Constants.R /\
+   a6c{2} = a6c'{2} * zMinusLastOmega{2} %% Constants.R /\
+   to_uint _21{1} = statePowerOfAlpha7Slot{2} /\
+   to_uint _23{1} = stateL0AtZSlot{2} /\
+   to_uint intermediateValue{1} = a7c{2} /\
+   a7c{2} = statePowerOfAlpha7Slot{2} * stateL0AtZSlot{2} %% Constants.R /\
+   to_uint ret{1} = (a6c{2} - a7c{2}) %% Constants.R /\
+   to_uint lnMinusOneAtZ{1} = stateLnMinusOneAtZSlot{2} /\
+   Primops.memory{1} = modexp_memory_footprint m4 betaGamma{1} (DOMAIN_SIZE - W256.one) betaGammaPowered{1} /\
+   to_uint betaGammaPowered{1} = betaGammaPowered{2} /\ 0 <= betaGammaPowered{2} < Constants.R
+).
+call (modexp_low_equiv_mid m4 bg (DOMAIN_SIZE - W256.one)).
+skip. progress. rewrite /DOMAIN_SIZE. by progress.
+exists* betaGammaPowered{1}. elim* => bgp.
+pose m5 := modexp_memory_footprint m4 bg (DOMAIN_SIZE - W256.one) bgp.
+
+seq 1 0: (#pre /\ to_uint alphaPower8{1} = statePowerOfAlpha8Slot{2}).
+call{1} (ConcretePrimops.mload_pspec m5 STATE_POWER_OF_ALPHA_8_SLOT).
+skip. progress. rewrite /m5 /m4 /m3 /m2 /m1 /modexp_memory_footprint. progress.  
+rewrite load_store_diff /STATE_POWER_OF_ALPHA_7_SLOT /STATE_Z_MINUS_LAST_OMEGA_SLOT /STATE_L_N_MINUS_ONE_AT_Z_SLOT /STATE_POWER_OF_ALPHA_8_SLOT. by progress. by progress.
+do 13! (rewrite load_store_diff; try by progress). 
+rewrite /STATE_BETA_GAMMA_PLUS_GAMMA_SLOT. by progress.
+rewrite load_store_diff /STATE_BETA_PLUS_ONE_SLOT. by smt(). by smt(). by smt().
+
+seq 1 0: (#pre /\ to_uint _27{1} = (stateLnMinusOneAtZSlot{2} * betaGammaPowered{2}) %% Constants.R).
+wp. skip. rewrite /mulmod. progress. rewrite W256.to_uint_small. progress. by smt. by smt.
+rewrite H15. smt.
+
+seq 1 1: (#pre /\ to_uint subtrahend{1} = a8c{2} /\
+  a8c{2} = (statePowerOfAlpha8Slot{2} * stateLnMinusOneAtZSlot{2} * betaGammaPowered{2}) %% Constants.R).
+wp. skip. rewrite /mulmod. progress. rewrite W256.to_uint_small. progress. by smt. by smt.
+rewrite H19 H18. rewrite W256.to_uint_small. progress. by smt.
+
+wp. skip. progress. exists (to_uint lastOmega{1}) (to_uint betaGammaPowered{1}). progress.
+rewrite /addmod. progress. rewrite W256.to_uint_small. progress. by smt. by smt.
+pose lala := (to_uint (mload m STATE_POWER_OF_ALPHA_6_SLOT) *
+ ((to_uint (mload m PROOF_LOOKUP_S_POLY_OPENING_AT_Z_OMEGA_SLOT) *
+   to_uint (mload m STATE_BETA_LOOKUP_SLOT) + to_uint betaGamma{1}) %%
+  Constants.R) *
+ to_uint (mload m PROOF_LOOKUP_GRAND_PRODUCT_OPENING_AT_Z_OMEGA_SLOT) %%
+ Constants.R * to_uint zMinusLastOmega{1} %% Constants.R -
+ to_uint intermediateValue{1}).
+have ->: (lala - to_uint subtrahend{1}) %% Constants.R = (lala + (Constants.R - to_uint subtrahend{1})) %% Constants.R. smt().
+rewrite to_uintB. smt timeout=10. rewrite /lala H14. smt.
+smt(). smt(). smt(). smt(). smt(). smt(). smt(). smt().
+qed.
